theories/Hoare.v
@@ -1,0 +1,327 @@
+(**
+
+This file formalizes Hoare Logic:
+
+- heap entailement, written [H ==> H'],
+- definition of Hoare triple (total correctness)
+- consequence rule
+- rule for term constructs.
+
+It does not include reasoning rules for primitive operations on the heap,
+because these are more naturally expressed directly in Separation Logic.
+
+Author: Arthur Charguéraud.
+License: MIT.
+
+*)
+
+Set Implicit Arguments.
+From Sep Require Export Semantics.
+Open Scope fmap_scope.
+
+
+(* ********************************************************************** *)
+(** * Entailment *)
+
+(** The definition of entailment is polymorphic in the type of heaps,
+    which could be state, but also more elaborated structures in
+    extensions of Separation Logic (e.g. with time credits). *)
+
+
+(* ---------------------------------------------------------------------- *)
+(* ** Predicate extensionality, specialized to heap predicates *)
+
+(** Predicate extensionality follows from functional extensional
+    and propositional extensionality, which we take as axiom
+    (in TLC's LibAxioms file). *)
+
+Lemma hprop_extens : forall A (H1 H2:A->Prop),
+  (forall h, H1 h <-> H2 h) ->
+  (H1 = H2).
+Proof using.
+  introv M. applys fun_ext_1. intros h. applys* prop_ext.
+Qed.
+
+(* ---------------------------------------------------------------------- *)
+(* ** Definition of entailment *)
+
+(** [H1 ==> H2] is defined as [forall h, H1 h -> H2 h]. *)
+
+Definition himpl A (H1 H2:A->Prop) :=
+  forall x, H1 x -> H2 x.
+
+Notation "H1 ==> H2" := (himpl H1 H2)
+  (at level 55) : heap_scope.
+
+(** [Q1 ===> Q2] is defined as [forall x h, Q1 x h -> Q2 x h].
+    It is thus equivalent to [forall x, Q1 x ==> Q2 x].
+    Thus, invoking [intro] on a [===>] goal leaves a [==>] goal. *)
+
+Definition qimpl A B (Q1 Q2:A->B->Prop) :=
+  forall r, himpl (Q1 r) (Q2 r).
+
+Notation "Q1 ===> Q2" := (qimpl Q1 Q2)
+  (at level 55) : heap_scope.
+
+Open Scope heap_scope.
+
+
+(* ---------------------------------------------------------------------- *)
+(* ** Properties of entailment *)
+
+Section HimplProp.
+Variable A : Type.
+Implicit Types H : A -> Prop.
+
+Hint Unfold himpl.
+
+(** Entailment is reflexive, symmetric, transitive *)
+
+Lemma himpl_refl : forall H,
+  H ==> H.
+Proof using. intros h. auto. Qed.
+
+Lemma himpl_trans : forall H2 H1 H3,
+  (H1 ==> H2) ->
+  (H2 ==> H3) ->
+  (H1 ==> H3).
+Proof using. introv M1 M2. intros h H1h. eauto. Qed.
+
+Lemma himpl_antisym : forall H1 H2,
+  (H1 ==> H2) ->
+  (H2 ==> H1) ->
+  (H1 = H2).
+Proof using. introv M1 M2. applys pred_ext_1. intros h. iff*. Qed.
+
+(** Paragraphe of the definition, used by tactics *)
+
+Lemma himpl_inv : forall H1 H2 (h:A),
+  (H1 ==> H2) ->
+  (H1 h) ->
+  (H2 h).
+Proof using. auto. Qed.
+
+(** Reformulation of reflexivity, used by tactics *)
+
+Lemma himpl_of_eq : forall H1 H2,
+  H1 = H2 ->
+  H1 ==> H2.
+Proof. intros. subst. applys~ himpl_refl. Qed.
+
+Lemma himpl_of_eq_sym : forall H1 H2,
+  H1 = H2 ->
+  H2 ==> H1.
+Proof. intros. subst. applys~ himpl_refl. Qed.
+
+End HimplProp.
+
+Arguments himpl_of_eq [A] [H1] [H2].
+Arguments himpl_of_eq_sym [A] [H1] [H2].
+Arguments himpl_antisym [A] [H1] [H2].
+
+Hint Resolve himpl_refl.
+
+(** Reflexivity for postconditions *)
+
+Lemma qimpl_refl : forall A B (Q:A->B->Prop),
+  Q ===> Q.
+Proof using. intros. hnfs*. Qed.
+
+Hint Resolve qimpl_refl.
+
+
+(* ---------------------------------------------------------------------- *)
+(* ** Tactic [himpl_fold] *)
+
+(** [himpl_fold] applies to a goal of the form [H1 h].
+    It searches the context for an assumption of the from [H2 h],
+    then replaces the goal with [H1 ==> H2].
+    It also deletes the assumption [H2 h]. *)
+
+Ltac himpl_fold_core tt :=
+  match goal with N: ?H ?h |- _ ?h =>
+    applys himpl_inv N; clear N end.
+
+Tactic Notation "himpl_fold" := himpl_fold_core tt.
+Tactic Notation "himpl_fold" "~" := himpl_fold; auto_tilde.
+Tactic Notation "himpl_fold" "*" := himpl_fold; auto_star.
+
+
+(* ********************************************************************** *)
+(** * Definition of Hoare triples *)
+
+Definition hoare (t:trm) (H:state->Prop) (Q:val->state->Prop) :=
+  forall h, H h -> exists h' v, eval h t h' v /\ Q v h'.
+
+Implicit Types H : state->Prop.
+Implicit Types f : bind.
+Implicit Types v w : val.
+Implicit Types t : trm.
+Implicit Types vs : vals.
+
+
+(* ********************************************************************** *)
+(** * Hoare structural rules *)
+
+Lemma hoare_conseq : forall t H' Q' H Q,
+  hoare t H' Q' ->
+  H ==> H' ->
+  Q' ===> Q ->
+  hoare t H Q.
+Proof using.
+  introv M MH MQ HF. forwards (h'&v&R&K): M h.
+  { himpl_fold~. }
+  exists h' v. splits~. { himpl_fold. auto. }
+Qed.
+
+Lemma hoare_named_heap : forall t H Q,
+  (forall h, H h -> hoare t (= h) Q) ->
+  hoare t H Q.
+Proof using. introv M. intros h Hh. applys* M. Qed.
+
+
+(* ********************************************************************** *)
+(** * Hoare rules for term constructs *)
+
+Lemma hoare_evalctx : forall C t1 H Q Q1,
+  evalctx C ->
+  hoare t1 H Q1 ->
+  (forall v, hoare (C v) (Q1 v) Q) ->
+  hoare (C t1) H Q.
+Proof using.
+  introv HC M1 M2 Hh.
+  forwards* (h1'&v1&R1&K1): (rm M1).
+  forwards* (h2'&v2&R2&K2): (rm M2).
+  exists h2' v2. splits~. { applys~ eval_evalctx R2. }
+Qed.
+
+Lemma hoare_val : forall v H Q,
+  H ==> Q v ->
+  hoare (trm_val v) H Q.
+Proof using.
+  introv M. intros h Hh. exists h v. splits.
+  { applys eval_val. }
+  { himpl_fold~. }
+Qed.
+
+Lemma hoare_fixs : forall f xs t1 H Q,
+  xs <> nil ->
+  H ==> Q (val_fixs f xs t1) ->
+  hoare (trm_fixs f xs t1) H Q.
+Proof using.
+  introv N M. intros h Hh. exists___. splits.
+  { applys~ eval_fixs. }
+  { himpl_fold~. }
+Qed.
+
+Lemma hoare_constr : forall id vs H Q,
+  H ==> Q (val_constr id vs) ->
+  hoare (trm_constr id (trms_vals vs)) H Q.
+Proof using.
+  introv M. intros h Hh. exists h (val_constr id vs). splits.
+  { applys eval_constr. }
+  { himpl_fold~. }
+Qed.
+
+Lemma hoare_constr_trm : forall id ts t1 vs H Q Q1,
+  hoare t1 H Q1 -> 
+  (forall v, hoare (trm_constr id ((trms_vals vs)++(trm_val v)::ts)) (Q1 v) Q) ->
+  hoare (trm_constr id ((trms_vals vs)++t1::ts)) H Q.
+Proof using.
+  introv M1 M2. intros h Hh.
+  forwards* (h1'&v1&R1&K1): (rm M1).
+  forwards* (h2'&v2&R2&K2): (rm M2).
+  exists h2' v2. splits~. { applys~ eval_constr_trm R2. }
+Qed.
+
+Lemma hoare_let : forall z t1 t2 H Q Q1,
+  hoare t1 H Q1 ->
+  (forall v, hoare (subst1 z v t2) (Q1 v) Q) ->
+  hoare (trm_let z t1 t2) H Q.
+Proof using.
+  introv M1 M2 Hh.
+  forwards* (h1'&v1&R1&K1): (rm M1).
+  forwards* (h2'&v2&R2&K2): (rm M2).
+  exists h2' v2. splits~. { applys~ eval_let_trm R2. }
+Qed.
+
+Lemma hoare_if_bool : forall (b:bool) t1 t2 H Q,
+  hoare (if b then t1 else t2) H Q ->
+  hoare (trm_if b t1 t2) H Q.
+Proof using.
+  introv M1. intros h Hh. forwards* (h1'&v1&R1&K1): (rm M1).
+  exists h1' v1. splits~. { applys* eval_if. }
+Qed.
+
+Lemma hoare_if_trm : forall Q1 t0 t1 t2 H Q,
+  hoare t0 H Q1 ->
+  (forall v, hoare (trm_if v t1 t2) (Q1 v) Q) ->
+  hoare (trm_if t0 t1 t2) H Q.
+Proof using.
+  introv M1 M2. applys* hoare_evalctx (fun t0 => trm_if t0 t1 t2).
+  { constructor. }
+Qed.
+
+Lemma hoare_apps_funs : forall xs F vs t1 H Q,
+  F = (val_funs xs t1) ->
+  var_funs (length vs) xs ->
+  hoare (substn xs vs t1) H Q ->
+  hoare (trm_apps F vs) H Q.
+Proof using.
+  introv E N M. intros h Hh. forwards* (h'&v&R&K): (rm M).
+  exists h' v. splits~. { subst. applys* eval_apps_funs. }
+Qed.
+
+Lemma hoare_apps_fixs : forall xs (f:var) F vs t1 H Q,
+  F = (val_fixs f xs t1) ->
+  var_fixs f (length vs) xs ->
+  hoare (substn (f::xs) (F::vs) t1) H Q ->
+  hoare (trm_apps F vs) H Q.
+Proof using.
+  introv E N M. intros h Hh. forwards* (h'&v&R&K): (rm M).
+  exists h' v. splits~. { subst. applys* eval_apps_fixs. }
+Qed.
+
+Lemma hoare_while_raw : forall t1 t2 H Q,
+  hoare (trm_if t1 (trm_seq t2 (trm_while t1 t2)) val_unit) H Q ->
+  hoare (trm_while t1 t2) H Q.
+Proof using.
+  introv M Hh. forwards* (h1'&v1&R1&K1): (rm M).
+  exists h1' v1. splits~. { applys* eval_while. }
+Qed.
+
+Lemma hoare_for_raw : forall (x:var) (n1 n2:int) t3 H Q,
+  hoare (
+    If (n1 <= n2)
+      then (trm_seq (subst1 x n1 t3) (trm_for x (n1+1) n2 t3))
+      else val_unit) H Q ->
+  hoare (trm_for x n1 n2 t3) H Q.
+Proof using.
+  introv M Hh. forwards* (h1'&v1&R1&K1): (rm M).
+  exists h1' v1. splits~. { applys* eval_for. }
+Qed.
+
+Lemma hoare_match : forall v p t1 pts H Q,
+  (forall (G:ctx), Ctx.dom G = patvars p -> v = patsubst G p -> hoare (isubst G t1) H Q) ->
+  ((forall (G:ctx), Ctx.dom G = patvars p -> v <> patsubst G p) -> hoare (trm_match v pts) H Q) ->
+  hoare (trm_match v ((p,t1)::pts)) H Q.
+Proof using.
+  introv M1 M2 Hh. tests C: (exists (G:ctx), Ctx.dom G = patvars p /\ v = patsubst G p).
+  { destruct C as (G&DG&Ev). forwards* (h1'&v1&R1&K1): (rm M1).
+    exists h1' v1. splits~. { applys~ eval_match_yes R1. } }
+  { forwards* (h1'&v1&R1&K1): (rm M2).
+    exists h1' v1. splits~. { applys~ eval_match_no R1.
+      intros G HG. specializes C G. rew_logic in C. destruct* C. } }
+Qed.
+
+Lemma hoare_case_trm : forall t1 pts H Q Q1,
+  hoare t1 H Q1 -> 
+  (forall v, hoare (trm_match v pts) (Q1 v) Q) ->
+  hoare (trm_match t1 pts) H Q.
+Proof using.
+  introv M1 M2. intros h Hh.
+  forwards* (h1'&v1&R1&K1): (rm M1).
+  forwards* (h2'&v2&R2&K2): (rm M2).
+  exists h2' v2. splits~. { applys~ eval_match_trm R2. }
+Qed.
+
